README.md
@@ -8,16 +8,19 @@ The definition of the logical relation (**LR**) ressembles Loïc's in many ways,
 - Because of universe constraints and the fact that functors cannot be indexed by terms in Coq whereas it is possible in Agda, the relevant structures had to be parametrized by a type level and a recursor, and the module system had to be dropped out entirely.
 - Since Coq and Agda's positivity checking for inductive types is different, it turns out that **LR**'s definition, even though it does not use any induction-induction or induction-recursion in Agda, is not accepted in Coq. As such, the predicate over Π-types for **LR** has been modified compared to Agda. You can find a MWE of the difference in positivity checking in the two systems in [Positivity.v] and [Positivity.agda].
 
-In order to avoid some work on the syntax, this project uses the AST of [MetaCoq](https://metacoq.github.io), as well as some of its definitions (eg. substitution). While the AST has many nodes which are absent in the current formalization of MLTT, since these are not typable most proofs never have to consider them. Basically, only the proofs without typing assumptions have to be done for the whole AST, but most of these are done in MetaCoq already.
+In order to avoid some work on the syntax, this project uses the [Autosubst](https://github.com/uds-psl/autosubst-ocaml) project to generate syntax-related boilerplate.
 
 Building
 ===========
 
-The project builds with Coq version `8.15.2`. Once it has been installed, you can simply issue `make` in the root folder.
+The project builds with Coq version `8.15.2`. Once Coq has been installed, you can simply issue `make` in the root folder.
 
 
 File description
 ==========
+
+Utilities and AST
+---------
 
 | File | Description |
 |---|----|
@@ -25,23 +28,54 @@ File description
 [BasicAst] | Definitions preceding the definition of the AST itself: sorts, binder annotations…
 [AutoSubst/] | Abstract syntax tree, renamings, substitutions and many lemmas, generated using the [autosubst-ocaml] opam package.
 [Notations] | Notations used throughout the file. It can be used as an index for notations!
-[Context] | Context-related definitions: declaration, mapping over a context, find a type in a context…
 [Untyped] | Various useful definitions for defining the inference rules |
+
+Common typing-related definitions
+-------
+
+| File | Description |
+|---|----|
+[Context] | Context-related definitions: declaration, mapping over a context, find a type in a context…
 [UntypedReduction] | Definiton and basic properties of untyped reduction, used to define algorithmic typing.
 [Weakening] | Definition of a well-formed weakening, and some properties.
-[Substitution] | Definition of a well-formed substitution.
 [GenericTyping] | A generic notion of typing, used to define the logical relation, to be instantiated twice: once with the declarative version, and once with the algorithmic one.
+
+Declarative typing and its properties
+--------------
+
+| File | Description |
+|---|----|
 [DeclarativeTyping] | Defines the theory's typing rules in a declarative fashion, the current definition has a single universe as well as product types and eta-conversion for functions. |
 [Generation] | Contains generation theorems, giving a good inversion on term typing/reduction with a direct structural premise
 [Reduction] | Basic properties of reduction, enough to derive that declarative typing is an instance of generic typing. |
-[AlgorithmicTyping] | Definition of the second notion of typing : algorithmic typing (and algorithmic conversion together with it).
+
+Logical relation and its properties
+-----------
+
+| File | Description |
+|---|----|
 [LogicalRelation] | Contains the logical relation's (**LR**) definition. |
 | [LRInduction] | Defines the induction principles over **LR**. Because of universe constraints, **LR** needs two induction principles, one for each type levels. |
 | [Escape] | Contains a proof of the escape lemma for **LR** |
 | [Shapeview] | Technique to avoid considering non-diagonal cases for two reducibly convertible types. |
 [Reflexivity] | Reflexivity of the logical relation.
 [Irrelevance] | Irrelevance of the logical relation: two convertible types decode to equivalent predicates. Symmetry is a direct corollary. |
-[AlgorithmicTypingProperties] | Properties of the algorithmic typing, in order to derive the second instance of generic typing. |
+
+Algorithmic typing and its properties
+-----------------
+
+| File | Description |
+|---|----|
+[AlgorithmicTyping] | Definition of the second notion of typing : algorithmic typing (and algorithmic conversion together with it).
+[LogRelConsequences] | Consequences of the logical relation on declarative typing necessary to establish properties of algorithmic typing.
+[BundledAlgorithmicTyping] | Algorithmic typing bundled with its pre-conditions, and a tailored induction principle showing invariant preservation in the "algorithm".
+[AlgorithmicTypingProperties] | Properties of algorithmic typing, in order to derive the second instance of generic typing. |
+
+Miscellaneous
+-----------
+
+| File | Description |
+|---|----|
 | [Positivity.v] and [Positivity.agda] | Showcase the difference between Coq and Agda's positivity checkers. |
 
 [Utils]: ./theories/Utils.v
@@ -68,6 +102,8 @@ File description
 [Substitution]: ./theories/Substitution.v
 [AlgorithmicTyping]: ./theories/AlgorithmicTyping.v
 [AlgorithmicTypingProperties]: ./theories/AlgorithmicTypingProperties.v
+[LogRelConsequences]: ./theories/LogRelConsequences.v
+[BundledAlgorithmicTyping]: ./theories/BundledAlgorithmicTyping.v
 
 [autosubst-ocaml]: https://github.com/uds-psl/autosubst-ocaml
 [Positivity.agda]: ./theories/Positivity.agda
